Sanity restored to some extend, stage2 builds

tests/pkg/module/Module/Basic.lean
@@ -5,9 +5,126 @@ module
 /-- A definition. -/
 def f := 1
 
+#guard_msgs(drop warning) in
 /-- A theorem. -/
 theorem t : f = 1 := sorry
 
 theorem trfl : f = 1 := rfl
 
 @[expose] def fexp := 1
+
+def f_struct : Nat → Nat
+| 0 => 0
+| n + 1 => f_struct n
+termination_by structural n => n
+
+def f_wfrec : Nat → Nat
+| 0 => 0
+| n + 1 => f_wfrec n
+termination_by n => n
+
+@[expose] def f_exp_wfrec : Nat → Nat
+| 0 => 0
+| n + 1 => f_exp_wfrec n
+termination_by n => n
+
+@[inline] protected def Test.Option.map (f : α → β) : Option α → Option β
+  | some x => some (f x)
+  | none   => none
+
+
+/-- error: 'f.eq_def' is a reserved name -/
+#guard_msgs in
+def f.eq_def := 1
+
+/-- error: 'fexp.eq_def' is a reserved name -/
+#guard_msgs in
+def fexp.eq_def := 1
+
+/-- info: f.eq_def : f = 1 -/
+#guard_msgs in
+#check f.eq_def
+
+/-- info: f.eq_unfold : f = 1 -/
+#guard_msgs in
+#check f.eq_unfold
+
+/-- info: fexp.eq_def : fexp = 1 -/
+#guard_msgs in
+#check fexp.eq_def
+
+/-- info: fexp.eq_unfold : fexp = 1 -/
+#guard_msgs in
+#check fexp.eq_unfold
+
+/-- info: f_struct.eq_1 : f_struct 0 = 0 -/
+#guard_msgs in
+#check f_struct.eq_1
+
+/--
+info: f_struct.eq_def (x✝ : Nat) :
+  f_struct x✝ =
+    match x✝ with
+    | 0 => 0
+    | n.succ => f_struct n
+-/
+#guard_msgs in
+#check f_struct.eq_def
+
+/--
+info: f_struct.eq_unfold :
+  f_struct = fun x =>
+    match x with
+    | 0 => 0
+    | n.succ => f_struct n
+-/
+#guard_msgs(pass trace, all) in
+#check f_struct.eq_unfold
+
+/-- info: f_wfrec.eq_1 : f_wfrec 0 = 0 -/
+#guard_msgs(pass trace, all) in
+#check f_wfrec.eq_1
+
+/--
+info: f_wfrec.eq_def (x✝ : Nat) :
+  f_wfrec x✝ =
+    match x✝ with
+    | 0 => 0
+    | n.succ => f_wfrec n
+-/
+#guard_msgs in
+#check f_wfrec.eq_def
+
+/--
+info: f_wfrec.eq_unfold :
+  f_wfrec = fun x =>
+    match x with
+    | 0 => 0
+    | n.succ => f_wfrec n
+-/
+#guard_msgs in
+#check f_wfrec.eq_unfold
+
+/-- info: f_exp_wfrec.eq_1 : f_exp_wfrec 0 = 0 -/
+#guard_msgs in
+#check f_exp_wfrec.eq_1
+
+/--
+info: f_exp_wfrec.eq_def (x✝ : Nat) :
+  f_exp_wfrec x✝ =
+    match x✝ with
+    | 0 => 0
+    | n.succ => f_exp_wfrec n
+-/
+#guard_msgs in
+#check f_exp_wfrec.eq_def
+
+/--
+info: f_exp_wfrec.eq_unfold :
+  f_exp_wfrec = fun x =>
+    match x with
+    | 0 => 0
+    | n.succ => f_exp_wfrec n
+-/
+#guard_msgs in
+#check f_exp_wfrec.eq_unfold
