src/Lean/Elab/PreDefinition/PartialFixpoint/Eqns.lean
@@ -72,11 +72,7 @@ private def rwFixEq (mvarId : MVarId) : MetaM MVarId := mvarId.withContext do
 
 /-- Generate the "unfold" lemma for `declName`. -/
 def mkUnfoldEq (declName : Name) (info : EqnInfo) : MetaM Name := do
-  let isExposedDef ← withExporting do (·.hasValue) <$> getConstInfo declName
-  let baseName := declName
-  let mut name := Name.str baseName unfoldThmSuffix
-  unless isExposedDef do
-    name := mkPrivateName (← getEnv) name
+  let name := mkEqLikeNameFor (← getEnv) declName unfoldThmSuffix
   realizeConst declName name (doRealize name)
   return name
 where
@@ -108,7 +104,7 @@ where
       }
 
 def getUnfoldFor? (declName : Name) : MetaM (Option Name) := do
-  let name := Name.str declName unfoldThmSuffix
+  let name := mkEqLikeNameFor (← getEnv) declName unfoldThmSuffix
   let env ← getEnv
   if env.contains name then return name
   let some info := eqnInfoExt.find? env declName | return none
