tests/pkg/module/Module/ImportedAll.lean
@@ -22,3 +22,79 @@ but is expected to have type
 -/
 #guard_msgs in
 theorem v (x : Vector Unit f) (y : Vector Unit 1) : x = y := sorry
+
+
+
+/-- info: f.eq_def : f = 1 -/
+#guard_msgs in
+#check f.eq_def
+
+/-- info: f.eq_unfold : f = 1 -/
+#guard_msgs in
+#check f.eq_unfold
+
+/-- info: f_struct.eq_1 : f_struct 0 = 0 -/
+#guard_msgs in
+#check f_struct.eq_1
+
+/--
+info: f_struct.eq_def (x✝ : Nat) :
+  f_struct x✝ =
+    match x✝ with
+    | 0 => 0
+    | n.succ => f_struct n
+-/
+#guard_msgs in
+#check f_struct.eq_def
+
+/--
+info: f_struct.eq_unfold :
+  f_struct = fun x =>
+    match x with
+    | 0 => 0
+    | n.succ => f_struct n
+-/
+#guard_msgs in
+#check f_struct.eq_unfold
+
+/-- info: f_wfrec.eq_1 : f_wfrec 0 = 0 -/
+#guard_msgs in
+#check f_wfrec.eq_1
+
+/-- error: unknown identifier 'f_wfrec.eq_def' -/
+#guard_msgs in
+#check f_wfrec.eq_def
+
+/--
+info: f_wfrec.eq_unfold :
+  f_wfrec = fun x =>
+    match x with
+    | 0 => 0
+    | n.succ => f_wfrec n
+-/
+#guard_msgs in
+#check f_wfrec.eq_unfold
+
+/-- info: f_exp_wfrec.eq_1 : f_exp_wfrec 0 = 0 -/
+#guard_msgs in
+#check f_exp_wfrec.eq_1
+
+/--
+info: f_exp_wfrec.eq_def (x✝ : Nat) :
+  f_exp_wfrec x✝ =
+    match x✝ with
+    | 0 => 0
+    | n.succ => f_exp_wfrec n
+-/
+#guard_msgs in
+#check f_exp_wfrec.eq_def
+
+/--
+info: f_exp_wfrec.eq_unfold :
+  f_exp_wfrec = fun x =>
+    match x with
+    | 0 => 0
+    | n.succ => f_exp_wfrec n
+-/
+#guard_msgs in
+#check f_exp_wfrec.eq_unfold
